porting to the duplicated version of pmap

Java/src/Java/Func/JavaFunc.v
@@ -1,27 +1,17 @@
-Require Import ChargeCore.Open.Subst.
-Require Import ChargeCore.Open.Open.
-Require Import ChargeCore.Open.Stack.
-Require Import ChargeCore.Logics.BILogic.
-Require Import Charge.Views.ILogicView.
-Require Import Charge.Views.BILogicView.
-Require Import Charge.Views.SubstView.
-Require Import Charge.Views.EmbedView.
-
+Set Printing Universes.
 Require Import ExtLib.Core.RelDec.
 Require Import ExtLib.Data.Fun.
 Require Import ExtLib.Data.String.
 Require Import ExtLib.Data.Sum.
 Require Import ExtLib.Data.Positive.
-Require Import ExtLib.Data.SumN.
-Require Import ExtLib.Data.Map.FMapPositive.
 Require Import ExtLib.Tactics.Consider.
 
 Require Import MirrorCore.TypesI.
 Require Import MirrorCore.SymI.
 Require Import MirrorCore.Lemma.
 Require Import MirrorCore.Lambda.Expr.
-Require Import MirrorCore.Views.FuncView.
 Require Import MirrorCore.Views.ViewSumN.
+Require Import MirrorCore.Views.FuncView.
 Require Import MirrorCore.syms.SymEnv.
 Require Import MirrorCore.syms.SymSum.
 Require Import MirrorCore.syms.SymOneOf.
@@ -34,6 +24,16 @@ Require Import MirrorCore.Views.ApplicativeView.
 Require Import MirrorCore.Views.NatView.
 Require Import MirrorCore.Views.BoolView.
 Require Import MirrorCore.Views.StringView.
+
+Require Import ChargeCore.Open.Subst.
+Require Import ChargeCore.Open.Open.
+Require Import ChargeCore.Open.Stack.
+Require Import ChargeCore.Logics.BILogic.
+Require Import Charge.Views.ILogicView.
+Require Import Charge.Views.BILogicView.
+Require Import Charge.Views.SubstView.
+Require Import Charge.Views.EmbedView.
+
 
 Require Import Java.Logic.AssertionLogic.
 Require Import Java.Logic.SpecLogic.
@@ -55,22 +55,22 @@ Inductive java_func :=
 | pCmd (c : cmd)
 | pExpr (e : dexpr)
 | pFields (f : list string)
-          
+
 | pMethodSpec
 | pProgEq
 | pTriple
 | pTypeOf
 | pFieldLookup
 | pMethodLookup
-    
+
 | pPointsto
 | pNull
-    
+
 | pMethodBody
 | pMethodArgs
 | pMethodRet
-    
-    
+
+
 | pPlus
 | pMinus
 | pTimes
@@ -95,24 +95,24 @@ Definition typeof_java_func bf :=
   | pVal _ => Some tyVal
   | pExpr _ => Some tyDExpr
   | pFields _ => Some (tyList tyString)
-		      
+
   | pMethodSpec => Some (tyArr tyString (tyArr tyString (tyArr tyVarList
 		    	                                       (tyArr tyString (tyArr tySasn (tyArr tySasn tySpec))))))
   | pProgEq => Some (tyArr tyProg tySpec)
   | pTriple => Some (tyArr tySasn (tyArr tySasn (tyArr tyCmd tySpec)))
-		    
+
   | pTypeOf => Some (tyArr tyString (tyArr tyVal tyProp))
-		    
+
   | pFieldLookup => Some (tyArr tyProg (tyArr tyString (tyArr tyFields tyProp)))
   | pMethodLookup => Some (tyArr tyProg (tyArr tyString (tyArr tyString (tyArr tyMethod tyProp))))
-		    
+
   | pPointsto => Some (tyArr tyVal (tyArr tyString (tyArr tyVal tyAsn)))
   | pNull => Some tyVal
-		  
+
   | pMethodBody => Some (tyArr tyMethod tyCmd)
   | pMethodArgs => Some (tyArr tyMethod (tyList tyString))
   | pMethodRet => Some (tyArr tyMethod tyDExpr)
-		       
+
   | pPlus => Some (tyArr tyVal (tyArr tyVal tyVal))
   | pMinus => Some (tyArr tyVal (tyArr tyVal tyVal))
   | pTimes => Some (tyArr tyVal (tyArr tyVal tyVal))
@@ -131,21 +131,21 @@ Definition java_func_eq (a b : java_func) : option bool :=
   | pExpr e1, pExpr e2 => Some (e1 ?[ eq ] e2)
   | pFields f1, pFields f2 => Some (f1 ?[ eq ] f2)
   | pCmd c1, pCmd c2 => Some (c1 ?[ eq ]c2)
-	                     
+
   | pMethodSpec, pMethodSpec => Some true
   | pProgEq, pProgEq => Some true
   | pTriple, pTriple => Some true
-	                     
+
   | pTypeOf, pTypeOf => Some true
-	                     
+
   | pPointsto, pPointsto => Some true
   | pFieldLookup, pFieldLookup => Some true
   | pMethodLookup, pMethodLookup => Some true
-	                                 
+
   | pMethodBody, pMethodBody => Some true
   | pMethodArgs, pMethodArgs => Some true
   | pMethodRet, pMethodRet => Some true
-	                           
+
   | pNull, pNull => Some true
   | pPlus, pPlus => Some true
   | pMinus, pMinus => Some true
@@ -158,31 +158,30 @@ Definition java_func_eq (a b : java_func) : option bool :=
   | _, _ => None
   end.
 
-Global Instance RelDec_java_func : RelDec (@eq java_func) := 
-  {
-    rel_dec a b := match java_func_eq a b with 
-    	  	   | Some b => b 
-    		   | None => false 
-    		   end
-  }.
+Global Instance RelDec_java_func : RelDec (@eq java_func) :=
+{ rel_dec a b := match java_func_eq a b with
+    	  	 | Some b => b
+    		 | None => false
+    		 end
+}.
 
 Global Instance RelDec_Correct_java_func : RelDec_Correct RelDec_java_func.
 Proof.
   constructor.
   destruct x; destruct y; simpl;
   try solve [ try rewrite Bool.andb_true_iff ;
-              repeat rewrite rel_dec_correct; intuition congruence ].                  	
+              repeat rewrite rel_dec_correct; intuition congruence ].
 Qed.
 (*
 Definition set_fold_fun (x : String.string) (f : field) (P : sasn) :=
 	(liftn pointsto) (x/V) `f `null ** P.
 *)
 Definition java_func_symD bf :=
-  match bf as bf return match typeof_java_func bf with
+  match bf as bf return match typeof_java_func bf return Type@{Urefl} with
 			| Some t => typD t
 			| None => unit
 			end with
-    
+
   | pProg p => p
   | pMethod m => m
   | pVal v => v
@@ -192,20 +191,20 @@ Definition java_func_symD bf :=
   | pMethodSpec => method_spec
   | pProgEq => prog_eq
   | pTriple => triple
-                 
+
   | pTypeOf => typeof
-                 
+
   | pFieldLookup => field_lookup
   | pMethodLookup => method_lookup
-                       
+
   | pPointsto => pointsto
-                   
+
   | pNull => null
-               
+
   | pMethodBody => m_body
   | pMethodArgs => m_params
   | pMethodRet => m_ret
-                    
+
   | pPlus => eplus
   | pMinus => eminus
   | pTimes => etimes
@@ -216,12 +215,11 @@ Definition java_func_symD bf :=
   | pValEq => eeq
   end.
 
-Global Instance RSym_JavaFunc : SymI.RSym java_func := 
-  {
-    typeof_sym := typeof_java_func;
-    symD := java_func_symD;
-    sym_eqb := java_func_eq
-  }.
+Global Instance RSym_JavaFunc : SymI.RSym java_func :=
+{ typeof_sym := typeof_java_func;
+  symD := java_func_symD;
+  sym_eqb := java_func_eq
+}.
 
 Global Instance RSymOk_JavaFunc : SymI.RSymOk RSym_JavaFunc.
 Proof.
@@ -233,22 +231,26 @@ Proof.
   consider (c ?[ eq ] c0); intros; subst; intuition congruence.
   consider (e ?[ eq ] e0); intros; subst; intuition congruence.
   consider (f ?[ eq ] f0); intros; subst; intuition congruence.
-Qed.	
+Qed.
 
-Inductive list' (A : Type) :=
-  | nil' : list' A
-  | cons' : A -> list' A -> list' A.
+Inductive list' :=
+| nil' : list'
+| cons' : OneOfType.TypeR -> list' -> list'.
 
-Fixpoint list_to_pmap_aux {T : Type} (lst : list' T) (p : positive) : pmap T :=
+Fixpoint list_to_pmap_aux (lst : list') (p : positive)
+: OneOfType.pmap :=
   match lst with
-    | nil' => Empty
-    | cons' x xs => pmap_insert p x (list_to_pmap_aux xs (p + 1))
+  | nil' => OneOfType.Empty
+  | cons' x xs => OneOfType.pmap_insert p (list_to_pmap_aux xs (p + 1)) x
   end.
-  
-Definition list_to_pmap {T : Type} (lst : list' Type) := list_to_pmap_aux lst 1.
 
-Definition func_map : pmap Type :=
-	list_to_pmap (T := Type) 
+Definition list_to_pmap (lst : list') := list_to_pmap_aux lst 1.
+
+
+Set Printing Universes.
+
+Definition func_map : OneOfType.pmap :=
+	list_to_pmap
 	  (cons' java_func
           (cons' SymEnv.func
           (cons' (@ilfunc typ)
@@ -262,9 +264,11 @@ Definition func_map : pmap Type :=
           (cons' (@prod_func typ)
           (cons' (@eq_func typ)
           (cons' (@ap_func typ)
-          (cons' (@listOp_func typ) (nil' Type))))))))))))))).
+          (cons' (@listOp_func typ) nil')))))))))))))).
 
-Definition func := OneOf func_map.
+Definition func := OneOfType.OneOf func_map.
+
+Check @red_fold typ func.
 
 Global Instance JavaView_func : FuncView func java_func :=
   FuncViewPMap 1 func_map eq_refl.
@@ -301,7 +305,7 @@ Section MakeJavaFunc.
   Definition fCmd c : func:= f_insert (pCmd c).
   Definition fDExpr e : func:= f_insert (pExpr e).
   Definition fFields f : func:= f_insert (pFields f).
-  
+
   Definition fMethodSpec : func:= f_insert pMethodSpec.
   Definition fProgEq : func:= f_insert pProgEq.
   Definition fTriple : func:= f_insert pTriple.
@@ -310,11 +314,11 @@ Section MakeJavaFunc.
   Definition fMethodLookup : func:= f_insert pMethodLookup.
   Definition fPointsto : func:= f_insert pPointsto.
   Definition fNull : func:= f_insert pNull.
-  
+
   Definition fMethodBody : func:= f_insert pMethodBody.
   Definition fMethodArgs : func:= f_insert pMethodArgs.
-  Definition fMethodRet : func:= f_insert pMethodRet.	
-  
+  Definition fMethodRet : func:= f_insert pMethodRet.
+
   Definition fPlusE : func:= f_insert pPlus.
   Definition fMinusE : func:= f_insert pMinus.
   Definition fTimesE : func:= f_insert pTimes.
@@ -489,8 +493,8 @@ Require Import MirrorCore.Lambda.Ptrns.
       end.
 
   Definition ptrnTriple {A B C : Type}
-             (a : ptrn (expr typ func) A) 
-             (b : ptrn (expr typ func) B) 
+             (a : ptrn (expr typ func) A)
+             (b : ptrn (expr typ func) B)
              (c : ptrn (expr typ func) C) : ptrn (expr typ func) (A * B * C) :=
     pmap (fun a_b_c => let '(_, a, b, c) := a_b_c in (a, b, c))
          (app (app (app (inj (ptrn_view _ fptrnTriple)) a) b) c).
@@ -499,17 +503,17 @@ Require Import MirrorCore.Lambda.Ptrns.
   Definition mkFieldLookup P C f : expr typ func := App (App (App (Inj fFieldLookup) P) C) f.
   Definition mkTypeOf C x : expr typ func := App (App (Inj fTypeOf) C) x.
   Definition mkProgEq P : expr typ func := App (Inj fProgEq) P.
-  
-  Definition mkMethodBody (M : Method) : expr typ func := 
+
+  Definition mkMethodBody (M : Method) : expr typ func :=
     App (Inj fMethodBody) (Inj (fMethod M)).
-  Definition mkMethodArgs (M : Method) : expr typ func := 
+  Definition mkMethodArgs (M : Method) : expr typ func :=
     App (Inj fMethodArgs) (Inj (fMethod M)).
-  Definition mkMethodRet (M : Method) : expr typ func := 
+  Definition mkMethodRet (M : Method) : expr typ func :=
     App (Inj fMethodRet) (Inj (fMethod M)).
 
-	
+
   Definition mkExprList es :=
-    (fold_right (fun (e : dexpr) (acc : expr typ func) => 
+    (fold_right (fun (e : dexpr) (acc : expr typ func) =>
 		   mkCons tyExpr (Inj (fDExpr e)) acc) (mkNil tyExpr) es).
 
 Fixpoint evalDExpr (e : dexpr) : expr typ func :=
@@ -535,17 +539,17 @@ Section JavaFunc.
 
   Context {fs : Environment}.
 
-(* This needs to be parametric. It shouldn't be here 
+(* This needs to be parametric. It shouldn't be here
 Definition fs : @SymEnv.functions typ _ :=
   SymEnv.from_list
   	(@SymEnv.F typ _ (tyArr tyVal (tyArr (tyList tyVal) tyAsn)) List::
-  	 @SymEnv.F typ _ (tyArr tyVal (tyArr (tyList tyVal) tyAsn)) NodeList::nil). 
+  	 @SymEnv.F typ _ (tyArr tyVal (tyArr (tyList tyVal) tyAsn)) NodeList::nil).
 
 *)
 
-  Global Instance RSym_ilfunc : RSym (@ilfunc typ) := 
+  Global Instance RSym_ilfunc : RSym (@ilfunc typ) :=
 	  RSym_ilfunc ilops.
-  Global Instance RSym_bilfunc : RSym (@bilfunc typ) := 
+  Global Instance RSym_bilfunc : RSym (@bilfunc typ) :=
 	  RSym_bilfunc bilops.
   Global Instance RSym_embed_func : RSym (@embed_func typ) :=
 	  RSym_embed_func eops.
@@ -564,17 +568,17 @@ Definition fs : @SymEnv.functions typ _ :=
   Global Existing Instance RSymOk_sum.
 
   Require Import ExtLib.Structures.Applicative.
-  
+
   Local Instance Applicative_Fun A : Applicative (Fun A) :=
     { pure := fun _ x _ => x
       ; ap := fun _ _ f x y => (f y) (x y)
     }.
 
-  
+
   Definition RSym_sub_func (p : positive) :
-    RSym (match pmap_lookup' func_map p with 
-          | Some T => T 
-          | None => Empty_set 
+    RSym (match pmap_lookup' func_map p with
+          | Some T => T
+          | None => Empty_set
           end).
   Proof.
     destruct p; simpl; [| | apply _].
@@ -608,16 +612,16 @@ Definition fs : @SymEnv.functions typ _ :=
     induction p; simpl; intuition; apply RSym_Empty_set.
   Defined.
 
-  Instance RSymOk_Empty_set : RSymOk RSym_Empty_set := 
+  Instance RSymOk_Empty_set : RSymOk RSym_Empty_set :=
     {
       sym_eqbOk a b :=
-        match a return (match sym_eqb a b with 
-                        | Some true => a = b 
+        match a return (match sym_eqb a b with
+                        | Some true => a = b
                         | Some false => a <> b
                         | None => True
                         end) with
         end
-    
+
     }.
 
   Lemma RSymOk_sub_func (p : positive) : RSymOk (RSym_sub_func p).
@@ -654,7 +658,7 @@ Definition fs : @SymEnv.functions typ _ :=
   Defined.
 
   Global Instance RSym_func : RSym func := RSymOneOf func_map RSym_sub_func.
-  
+
   Global Instance RSymOk_func : RSymOk RSym_func := RSymOk_OneOf func_map RSym_sub_func RSymOk_sub_func.
 
   Global Instance Expr_expr : ExprI.Expr _ (expr typ func) := @Expr_expr typ func _ _ _.
@@ -674,8 +678,8 @@ Definition fs : @SymEnv.functions typ _ :=
   Global Instance SS : SubstI.Subst subst (expr typ func) :=
     @FMapSubst.SUBST.Subst_subst _.
   Global Instance SU : SubstI.SubstUpdate subst (expr typ func) :=
-    @FMapSubst.SUBST.SubstUpdate_subst _ _ _ _. 
-  Global Instance SO : SubstI.SubstOk SS := 
+    @FMapSubst.SUBST.SubstUpdate_subst _ _ _ _.
+  Global Instance SO : SubstI.SubstOk SS :=
     @FMapSubst.SUBST.SubstOk_subst typ RType_typ (expr typ func) _.
   Global Instance SUO :SubstI.SubstUpdateOk SU SO :=  @FMapSubst.SUBST.SubstUpdateOk_subst typ RType_typ (expr typ func) _ _.
 (*
@@ -689,9 +693,9 @@ Definition fs : @SymEnv.functions typ _ :=
   Qed.
 *)
 
-  Lemma evalDExpr_wt (e : dexpr) : 
+  Lemma evalDExpr_wt (e : dexpr) :
 	  typeof_expr nil nil (evalDExpr e) = Some tyExpr.
-  Proof. 
+  Proof.
     induction e.
     + simpl; reflexivity.
     + simpl; reflexivity.
@@ -706,10 +710,10 @@ Definition fs : @SymEnv.functions typ _ :=
   Qed.
 
   Definition is_pure : expr typ func -> bool :=
-    run_tptrn 
-      (pdefault 
+    run_tptrn
+      (pdefault
          (por (pmap (fun _ => true) (por (ptrnTrue ignore) (ptrnFalse ignore)))
-              (pmap (fun x => 
+              (pmap (fun x =>
                        match x with
                        | (tyPure, tySasn, tt) => true
                        | _ => false
@@ -718,10 +722,10 @@ Definition fs : @SymEnv.functions typ _ :=
          false).
 
   Definition mkPointstoVar x f e : expr typ func :=
-     mkAp tyVal tyAsn 
+     mkAp tyVal tyAsn
           (mkAp tyString (tyArr tyVal tyAsn)
                 (mkAp tyVal (tyArr tyString (tyArr tyVal tyAsn))
-                      (mkPure (tyArr tyVal (tyArr tyString (tyArr tyVal tyAsn))) 
+                      (mkPure (tyArr tyVal (tyArr tyString (tyArr tyVal tyAsn)))
                                (Inj fPointsto))
                       (App (Inj fStackGet) (mkString x)))
                 (mkPure tyString (mkString f)))
